@prefix cex: <http://purl.org/weso/ontology/computex#> .
@prefix dcterms: <http://purl.org/dc/terms/> .
@prefix qb: <http://purl.org/linked-data/cube#> .
@prefix owl: <http://www.w3.org/2002/07/owl#> .
@prefix rdf: <http://www.w3.org/1999/02/22-rdf-syntax-ns#> .
@prefix rdfs: <http://www.w3.org/2000/01/rdf-schema#> .
@prefix sdmx-concept: <http://purl.org/linked-data/sdmx/2009/concept#> .
@prefix skos: <http://www.w3.org/2004/02/skos/core#> .
@prefix wi-onto: <http://data.webfoundation.org/webindex/ontology/> .
@prefix wi-org: <http://data.webfoundation.org/webindex/organization/> .
@prefix wi-people:  <http://data.webfoundation.org/webindex/people/> .
@prefix xsd: <http://www.w3.org/2001/XMLSchema#> .


wi-onto:
    a owl:Ontology;
    owl:versionInfo "0.2";
    rdfs:label "Webindex ontology"@en;
    rdfs:comment "Vocabulary for describing index structures and observations."@en;
    dcterms:created "2012-06-07"^^xsd:date;
    dcterms:modified "2013-06-07"^^xsd:date;
    dcterms:title "Core Webindex ontology"@en;
    dcterms:author wi-people:Labra , wi-people:Chema, wi-org:WESO ;
    dcterms:publisher  wi-org:WebFoundation;
    dcterms:contributor  wi-people:Hania, wi-people:Jules ;
    dcterms:license <http://opendatacommons.org/licenses/by/1.0/> .

wi-onto:Observation a owl:Class ; a rdfs:Class ;
             rdfs:label "Observation" ;
             rdfs:comment "An observation" .


wi-onto:Indicator a owl:Class ; a rdfs:Class ;
             rdfs:label "Indicator" ;
             rdfs:comment "A given indicator. Several indicators make a Component" ;
             skos:broader "Component" .

wi-onto:PrimaryIndicator a owl:Class, rdfs:Class;
	rdfs:subClassOf wi-onto:Indicator ;
	rdfs:label "Primary Indicator"@en ;
	rdfs:comment "Primary indicator is an indicator defined by the Webfoundation."@en;
.

wi-onto:SecondaryIndicator a owl:Class, rdfs:Class;
	rdfs:subClassOf wi-onto:Indicator ;
	rdfs:label "Secondary Indicator"@en ;
	rdfs:comment "This indicator is established by third parties such as ITU, UN, etc. Its observations are part of a component."@en;
.

wi-onto:ExternalIndicator a owl:Class, rdfs:Class;
	rdfs:subClassOf wi-onto:Indicator ;
	rdfs:label "External Indicator"@en ;
	rdfs:comment "This indicator is established by third parties such as Worldbank but its observations are not part of a component."@en;
.


wi-onto:Component a owl:Class ; a rdfs:Class ;
           rdfs:label "Component" ;
           rdfs:comment "An aggregation of several indicators" ;
           skos:broader :SubIndex .


wi-onto:SubIndex a owl:Class ; a rdfs:Class ;
          rdfs:label "A subindex" ;
          .


wi-onto:SheetData a owl:Class, rdfs:Class;
	rdfs:subClassOf skos:Concept ;
	rdfs:label "Sheet data"@en;
.

wi-onto:Raw a wi-onto:SheetData ;
	rdfs:label "Raw data"@en ;
	rdfs:comment "Raw data values that have been collected from a datasource without any normalisation process."@en ;
.

wi-onto:Imputed a wi-onto:SheetData ;
	rdfs:label "Imputed data"@en ;
	rdfs:comment "Data values that have been processed from their raw version to generate an imputed version."@en ;
.





